

# Logical Definitions

## Modus Ponens

$$\begin{array}{c} A \rightarrow B \\ B \\ \hline A \end{array}$$

First click Modus Ponens - to see the mathematical definition

Here is my understanding... essentially, with Modus Ponens - we assume the case where A implies B, i.e., “if 2+2 = 4, then 4 - 2 = 2”. In this scenario, if we just assume B is **true**, then we don’t need to worry about A becuae logically if B is **true**, then A **MUST** be **true** and here is the proof of that.

*Proof:*

$$\rightarrow ((A \rightarrow B) \wedge B) \rightarrow A$$

$$\rightarrow A \rightarrow B \equiv \neg A \vee B \text{ (By implication as disjunction)}$$

$$\rightarrow ((\neg A \vee B) \wedge B) \rightarrow A$$

$$\rightarrow \neg ((\neg A \vee B) \wedge B) \vee A \text{ (By implication as disjunction)}$$

{ Subroutine }:

$$\neg ((\neg A \vee B) \wedge B) \equiv \neg (\neg (A) \vee B) \vee \neg B \text{ (By De Morgan's Law)}$$
$$\neg (\neg (A) \vee B) \equiv A \wedge \neg B \text{ (By De Morgan's Law)}$$
$$A \wedge \neg B \equiv \perp \text{ (Since we asuumed } A \wedge B = \top \text{)}$$

---

$$\therefore \perp \vee \neg B \equiv \perp \text{ (Since we assumed } B = \top \text{)}$$

$$\rightarrow \perp \vee A \rightarrow A \text{ (By Law of Excluded Middle)}$$

---

$$\therefore ((A \rightarrow B) \wedge B) \rightarrow A \equiv A$$

□

A	⊥	B	¬B	⊥ ∨ A	A ∨ ¬B
T	F	T	F	T	T
T	F	F	T	T	T
F	F	T	F	F	F
F	F	F	T	F	T

# Modus Tollens

$$\begin{array}{l} A \rightarrow B \\ \neg B \\ \hline \neg A \end{array}$$

First click Modus Tollens - to see the mathematical definition

However, here is my interpretation of Modus Tollens. Basically if you know anything about logic - you know that the contrapositive is the logical equivalent to implication. This is the closest relation I can think of when thinkin with respect to Modus Tollens.

Here is the proof:

*Proof:*

$\rightarrow$  *Claim:*  $A \rightarrow B \leftrightarrow \neg B \rightarrow \neg A$

$\rightarrow$ 

A	$\neg A$	B	$\neg B$	$A \rightarrow B$	$\neg B \rightarrow \neg A$
T	F	T	F	T	T
T	F	F	T	F	F
F	T	T	F	T	T
F	T	F	T	T	T

□

# Hypothetical Syllogism

$$\begin{array}{l} A \rightarrow B \\ B \rightarrow C \\ \hline A \rightarrow C \end{array}$$

First click Hypothetical Syllogism - to see the mathematical definition

One way I look at Hypothetical Syllogism is the transitivity rule. Pretty much if you know about mathematical functions then you should know about the transitivity rule. If not here is a scenario, if you have  $A \leq B$   $B \leq C$  - then you can conclude  $A \leq C$ .